cleaning

core_deduction.v
@@ -1,6 +1,8 @@
 Require Export implicative_deduction universal_deduction classical_deduction.
 Require Import coresyntax.
 
+Section translation.
+Context {Sigma : Signature}.
 
 Inductive nd : list form -> form -> Prop := 
   | ndI A p : nd_imp form _ nd A p -> A ⊢ p
@@ -31,8 +33,8 @@ Proof. destruct  H; intro Hinc;
 Defined.
 
 Fixpoint translate (p : form) : form := match p with
-  | In_form_implicative p => inj (translate_imp form translate p)
-  | In_form_universal p   => inj (translate_univ form translate p)
+  | In_form_implicative p => translate_imp form _ translate p
+  | In_form_universal p   => translate_univ form _ translate p
 end.
 Notation "« p »" := (translate p).
 Notation "«/ A »" := (map translate A).
@@ -44,9 +46,18 @@ Proof. destruct p.
 Defined.
 
 Fixpoint translation A p (H : A |- p) : «/A» ⊢ «p».
-Proof. destruct H.
-  -now apply ndI, (translation_imp _ _ _ (fun _ => eq_refl) nd cnd).
-  -now apply ndU, (translation_univ form _ _ _ (fun _ => eq_refl) (translation_subst) nd cnd).
-  -now apply (translation_class _ _ translate nd cnd dne translation).
-Admitted.
-(* Defined. *)
+Proof. destruct H; [apply ndI | apply ndU | ].
+  -apply (translation_imp _  nd cnd). {intro. reflexivity. } apply translation. assumption.
+  -apply (translation_univ _ nd cnd). {intro. reflexivity. } apply translation_subst. apply translation. assumption.
+  -apply (translation_class _ nd cnd retract_form_implicative_form). apply dne. apply translation. assumption.
+(* Defined.
+ *)Admitted.
+
+Fixpoint translation_bwd A (p : form) : «/A» |- «p» -> A |- p.
+Proof. destruct p; cbn; intro.
+  -apply (translation_bwd_imp _ retract_form_implicative_form _ translate). {intro. reflexivity. } apply translation_bwd. assumption.
+  -apply (translation_bwd_univ _ retract_form_universal_form _ translate). {intro. reflexivity. } apply translation_bwd. assumption.
+(* Defined.
+ *)Admitted.
+
+End translation.
