disjunctive_deduction.v
@@ -1,6 +1,6 @@
 Require Export unscoped header_extensible.
-
 Require Export disjunctivesyntax implicativesyntax.
+Require Import classical_deduction implicative_deduction.
 
 Reserved Notation "A ⊢ p" (at level 70).
 Reserved Notation "A ⊢D p" (at level 70).
@@ -21,7 +21,6 @@ Section Disjunctive.
     | ndDI2 p q : A ⊢ q -> A ⊢D p ∨ q
     | ndDE p q r: A ⊢ p ∨ q -> p::A ⊢ r -> q::A ⊢ r -> A ⊢D r
   where "A ⊢D p" := (nd_disj A p).
-  Variable agree : forall A p, A ⊢D p -> A ⊢ p.
 
   Variable weakening : forall A B p, A ⊢ p -> incl A B -> B ⊢ p.
   Lemma weakening_disj A B p : A ⊢D p -> incl A B -> B ⊢D p.
@@ -40,6 +39,18 @@ Section Disjunctive.
   Notation "« p »" := (translate p).
   Notation "«/ A »" := (map translate A).
 
+  Variable agree : forall A p, A ⊢D p -> A ⊢ p.
+  Variable dne : forall A p, A ⊢ (¬¬p) -> A ⊢ p.
+  Variable dni : forall A p, A ⊢ p -> A ⊢ (¬¬p).
+  Variable imp_nd : forall A p, nd_imp _ _ nd A p -> A ⊢ p.
+  Variable translation_inj : forall p, «inj p» = translate_disj  p.
+  Variable translation_bwd : forall A p, A ⊢ «p» -> A ⊢ p.
+  Lemma translation_bwd_disj A p: A ⊢ (translate_disj p) -> A ⊢D inj p.
+  Proof. destruct p; cbn.  intro. apply dne in H. apply (ndDE _ _ _ (f ∨ f0)) in H. assumption.
+    -apply agree, ndDI1, translation_bwd, imp_nd, ndHyp. now left.
+    -apply agree, ndDI2, translation_bwd, imp_nd, ndHyp. now left.
+  Defined.
+
   Variable subst_form : (fin -> term) -> form -> form.
   Variable subst_form_inj : forall sigma p, subst_form sigma (inj p) = subst_form_disjunctive _ subst_form _ sigma p.
   Variable subst_dn : forall sigma p, subst_form sigma (¬¬p) = ¬¬(subst_form sigma p).
@@ -55,34 +66,40 @@ Section translation.
   Notation "A ⊢[ nd ] p" := (@nd_disj _ _ nd A p) (at level 70).
   Context {Sigma : Signature}.
 
-  Require Import classical_deduction.
   Variable form : Type.
+  Variable nd : list form -> form -> Prop.
+  Variable cnd : list form -> form -> Prop.
   Variable retract : retract (form_disjunctive form) form.
   Variable retract_implicative : included form_implicative form.
 
   Variable translate : form -> form.
   Notation "« p »" := (translate p).
   Notation "«/ A »" := (map translate A).
-
   Variable translation_inj : forall p, «inj p» = (translate_disj _ _  _ translate p).
 
-
-  Variable nd : list form -> form -> Prop.
-  Variable cnd : list form -> form -> Prop.
 
   Variable embed : forall A p, nd A p -> cnd A p.
   Lemma embed_disj A p : A ⊢[nd] p -> A ⊢[cnd] p.
   Proof. destruct 1; [ apply ndDI1 | apply ndDI2 | apply (ndDE _ _ _ _ p q) ]; now apply embed.
   Defined.
 
+  Variable imp_nd : forall A p, nd_imp form _ (nd_disj _ _ nd) A p -> A ⊢[nd] p.
+  Variable weakening : forall A B p, nd A p -> incl A B -> nd B p.
+
+  Lemma dn_int_disj A p: A ⊢[nd] p -> A ⊢[nd] (¬¬p).
+  Proof. intro. apply imp_nd, ndII, imp_nd, (ndIE _ _ _ _ p).
+    -apply imp_nd, ndHyp. now left.
+    -now apply (weakening_disj _ _ _ weakening A), incl_tl.
+  Qed.
+
+  Variable disj_cnd : forall A p, cnd A p -> A ⊢[cnd] p.
   Variable translation : forall A p, cnd A p -> nd «/A» «p».
   Lemma translation_disj A p: A ⊢[cnd] p -> «/A» ⊢[nd] «p».
-  Proof. Admitted.
+  Proof. destruct 1.
+    -rewrite translation_inj. cbn. now apply dn_int_disj, ndDI1, translation.
+    -rewrite translation_inj. cbn. now apply dn_int_disj, ndDI2, translation.
+    -apply (ndDE _ _ _ _ «p» «q»).
 
-  Variable subst_form : (fin -> term) -> form -> form.
-  Variable translation_subst : forall sigma q, «subst_form sigma q» = subst_form sigma «q».
-  Lemma translation_subst_disj sigma q: «subst_form sigma (inj q)» = subst_form sigma «inj q».
-  Proof. destruct q; repeat now rewrite translation_subst.
-  Defined.
+ Admitted.
 
 End translation.
