existential_deduction.v
@@ -1,6 +1,6 @@
 Require Export unscoped header_extensible.
-
 Require Export existentialsyntax implicativesyntax.
+Require Import classical_deduction implicative_deduction.
 
 Reserved Notation "A ⊢ p" (at level 70).
 Reserved Notation "A ⊢E p" (at level 70).
@@ -21,7 +21,6 @@ Section Existential.
     | ndEI p t : A ⊢ subst_form (scons t (var_term)) p -> A ⊢E (∃ p)
     | ndEE p q : A ⊢ (∃ p) -> p :: A ⊢ q -> A ⊢E q
   where "A ⊢E p" := (nd_exst A p).
-  Variable agree : forall A p, A ⊢E p -> A ⊢ p.
 
   Variable weakening : forall A B p, A ⊢ p -> incl A B -> B ⊢ p.
   Lemma weakening_exst A B p : A ⊢E p -> incl A B -> B ⊢E p.
@@ -36,8 +35,21 @@ Section Existential.
   Definition translate_exst (p : form_existential form) : _ := match p with
     | Exist _ q => ¬¬(∃ (translate q))
   end.
+  Notation "« p »" := (translate p).
+  Notation "«/ A »" := (map translate A).
 
-End Existential.
+  Variable agree : forall A p, A ⊢E p -> A ⊢ p.
+  Variable dne : forall A p, A ⊢ (¬¬p) -> A ⊢ p.
+  Variable dni : forall A p, A ⊢ p -> A ⊢ (¬¬p).
+  Variable subst_var: forall p, subst_form (var_term 0, var_term) p = p.
+  Variable imp_nd : forall A p, nd_imp _ _ nd A p -> A ⊢ p.
+  Variable translation_inj : forall p, «inj p» = translate_exst  p.
+  Variable translation_bwd : forall A p, A ⊢ «p» -> A ⊢ p.
+  Lemma translation_bwd_disj A p: A ⊢E (translate_exst p) -> A ⊢E inj p.
+  Proof. destruct p; cbn. intro. apply agree, dne in H. apply (ndEE _ _ (∃ f)) in H. assumption.
+    -apply agree, (ndEI _ _ (var_term 0)). rewrite subst_var. apply translation_bwd, imp_nd, ndHyp. now left.
+  Defined.
+
 
   Variable subst_form_inj : forall sigma p, subst_form sigma (inj p) = subst_form_existential _ subst_form _ sigma p.
   Variable subst_dn : forall sigma p, subst_form sigma (¬¬p) = ¬¬(subst_form sigma p).
@@ -47,37 +59,43 @@ End Existential.
     rewrite subst_form_inj. cbn. apply congr_Exist_; apply translation_subst. all: reflexivity.
   Defined.
 
+End Existential.
+
 Section translation.
   Context {Sigma : Signature}.
 
   Variable form : Type.
+  Variable nd : list form -> form -> Prop.
+  Variable cnd : list form -> form -> Prop.
   Variable subst_form : (fin -> term) -> form -> form.
   Variable retract_implicative : included form_implicative form.
   Variable retract_existential : included form_existential form.
   Variable translate : form -> form.
 
-  Notation "A ⊢[ nd ] p" := (@nd_exst _ _ subst_form nd A p) (at level 70).
+  Notation "A ⊢[ nd ] p" := (@nd_exst _ _ _ subst_form nd A p) (at level 70).
   Notation "« p »" := (translate p).
   Notation "«/ A »" := (map translate A).
 
   Variable translation_inj : forall p, «inj p» = translate_exst _ _ _ translate p.
   Variable translation_subst : forall sigma q, «subst_form sigma q» = subst_form sigma «q».
 
-  Lemma translation_subst_exst sigma q: «subst_form sigma (inj q)» = subst_form sigma «inj q».
-  Proof. destruct q. rewrite translation_subst. rewrite translation_inj. auto.
-  Defined.
-
-  Require Import classical_deduction.
-
-  Variable nd : list form -> form -> Prop.
-  Variable cnd : list form -> form -> Prop.
-
   Variable embed : forall A p, nd A p -> cnd A p.
   Lemma embed_exst A p : A ⊢[nd] p -> A ⊢[cnd] p.
   Proof. destruct 1. now apply (ndEI _ _ _ _ _ _ t), embed. apply (ndEE _ _ _ _ _ p); now apply embed.
   Defined.
 
+  Variable imp_nd : forall A p, nd_imp form _ (nd_exst _ _ subst_form nd) A p -> A ⊢[nd] p.
+  Variable weakening : forall A B p, nd A p -> incl A B -> nd B p.
+
+  Lemma dn_int_exst A p: A ⊢[nd] p -> A ⊢[nd] (¬¬p).
+  Proof. intro. apply imp_nd, ndII, imp_nd, (ndIE _ _ _ _ p).
+    -apply imp_nd, ndHyp. now left.
+    -now apply (weakening_exst _ _ _ _ weakening A), incl_tl.
+  Qed.
   Variable translation : forall A p, cnd A p -> nd «/A» «p».
   Lemma translation_exst A p: A ⊢[cnd] p -> «/A» ⊢[nd] «p».
-  Proof. Admitted.
+  Proof. destruct 1.
+    -rewrite translation_inj. apply dn_int_exst, (ndEI _ _ _ _ _ _ t). rewrite <- translation_subst. now apply translation.
+    -apply (ndEE _ _ _ _ _ «p»). admit. rewrite <- map_cons. now apply translation.
+  Admitted.
 End translation.
