implicative_deduction.v
@@ -1,10 +1,12 @@
 Require Export implicativesyntax.
+Require Import classical_deduction.
 
 Reserved Notation "A ⊢ p" (at level 70).
 Reserved Notation "A ⊢I p" (at level 70).
 
 
 Section implicative.
+  Context {Sigma : Signature}.
 
   Variable form : Type.
   Variable retract_implicative : included form_implicative form.
@@ -25,8 +27,6 @@ Section implicative.
     | ndIE p q : A ⊢ p ~> q -> A ⊢ p -> A ⊢I q
   where "A ⊢I p" := (nd_imp A p).
 
-(* Variable agree : forall A p, A ⊢I p -> A ⊢ p. *)
-
   Variable weakening : forall A B p, A ⊢ p -> incl A B -> B ⊢ p.
   Lemma weakening_imp A B p : A ⊢I p -> incl A B -> B ⊢I p.
   Proof. intro. revert B. destruct H; intros B Hinc;
@@ -39,15 +39,21 @@ Section implicative.
 
 
   Variable translate : form -> form.
+  Notation "« p »" := (translate p).
+  Notation "«/ A »" := (map translate A).
   Definition translate_imp (p : form_implicative form) : _ := match p with
     | Fal _ => ⊥
     | Impl _ p q => «p» ~> «q»
   end.
 
-End implicative.
-
   Variable translation_inj : forall p, «inj p» = translate_imp  p.
-  Variable agree : forall A p, A ⊢I p -> A ⊢ p.  Variable subst_form : (fin -> term) -> form -> form.
+
+  Variable translation_bwd : forall A p,  «/A» ⊢ «p» -> A ⊢ p.
+  Lemma translation_bwd_imp A p: «/A» ⊢ translate_imp p -> A ⊢ inj p.
+  Proof. destruct p; cbn; intro; apply translation_bwd; rewrite translation_inj; auto.
+  Defined.
+
+  Variable subst_form : (fin -> term) -> form -> form.
   Variable subst_form_inj : forall sigma p, subst_form sigma (inj p) = subst_form_implicative _ subst_form _ sigma p.
   Variable translation_subst : forall sigma q, «subst_form sigma q» = subst_form sigma «q».
   Lemma translation_subst_imp sigma p :  « subst_form_implicative _ subst_form _ sigma p » = subst_form sigma (translate_imp p).
@@ -56,45 +62,40 @@ End implicative.
     -rewrite subst_form_inj. unfold Impl_. rewrite translation_inj. cbn. apply congr_Impl_; apply translation_subst.
   Defined.
 
+End implicative.
+
 Notation "A ⊢I p" := (nd_imp A p) (at level 70).
 
 Section translation.
-  Notation "A ⊢[ nd ] p" := (@nd_imp _ _ nd A p) (at level 70).
   Context {Sigma : Signature}.
 
+  Notation "A ⊢[ nd ] p" := (@nd_imp _ _ nd A p) (at level 70).
   Variable form : Type.
+  Variable nd : list form -> form -> Prop.
+  Variable cnd : list form -> form -> Prop.
+
   Variable retract_implicative : included form_implicative form.
 
   Variable translate : form -> form.
   Notation "« p »" := (translate p).
   Notation "«/ A »" := (map translate A).
 
-  Variable translation_inj : forall p, «inj p» = inj (translate_imp _ translate p).
-
-
-  Require Import classical_deduction.
-
-  Variable nd : list form -> form -> Prop.
-  Variable cnd : list form -> form -> Prop.
 
   Variable embed : forall A p, nd A p -> cnd A p.
   Lemma embed_imp A p : A ⊢[nd] p -> A ⊢[cnd] p.
   Proof. destruct 1; [ now apply ndHyp | now apply ndExp, embed | now apply ndII, embed | ]. apply (ndIE _ _ _ _ p); now apply embed.
   Defined.
 
+  Variable translation_inj : forall p, «inj p» = translate_imp _ _ translate p.
+
   Variable translation : forall A p, cnd A p -> nd «/A» «p».
   Lemma translation_imp A p: A ⊢[cnd] p -> «/A» ⊢[nd] «p».
   Proof. destruct 1.
-    +now apply ndHyp, in_map.
-    +apply translation in H. rewrite translation_inj in H. cbn in H. now apply ndExp.
-    +rewrite translation_inj. cbn. apply ndII. rewrite <- map_cons. now apply translation.
-    +apply (ndIE _ _ _ _ «p»). 2: now apply translation. {pose (translation_inj (Impl _ p q)). cbn in e. rewrite <- e. now apply translation. }
+    -now apply ndHyp, in_map.
+    -apply ndExp. apply translation in H. rewrite translation_inj in H. now cbn in H.
+    -rewrite translation_inj. cbn. apply ndII. rewrite <- map_cons. now apply translation.
+    -apply (ndIE _ _ _ _ «p»). 2:now apply translation. {pose (translation_inj (Impl _ p q)). cbn in e. rewrite <- e. now apply translation. }
   Defined.
 
-  Variable subst_form : (fin -> term) -> form -> form.
-  Variable translation_subst : forall sigma q, «subst_form sigma q» = subst_form sigma «q».
-  Lemma translation_subst_imp sigma q : «subst_form sigma (inj q)» = subst_form sigma «inj q».
-  Proof. destruct q; repeat now rewrite translation_subst.
-  Defined.
 
 End translation.
